work on updating toBytecodeProofs
everything up to compile_val

compiler/proofs/toBytecodeProofsScript.sml
@@ -224,9 +224,9 @@ val env_renv_def = Define`
      Cenv renv)`
 
 val Cenv_bs_def = Define`
-  Cenv_bs rd Cmenv s Cenv (menv:string|->ctenv) (renv:ctenv) sz bs ⇔
+  Cenv_bs rd Cmenv s Cenv (menv:string|->num list) (renv:ctenv) sz bs ⇔
     env_renv rd sz bs Cenv renv ∧
-    fmap_rel (env_renv rd 0 bs) Cmenv menv ∧
+    fmap_rel (env_renv rd 0 bs) Cmenv (MAP CTDec o_f menv) ∧
     s_refs rd s bs`
 
 val Cenv_bs_syneq_store = store_thm("Cenv_bs_syneq_store",
@@ -1475,13 +1475,23 @@ val Cenv_bs_imp_incsz = store_thm("Cenv_bs_imp_incsz",
     ⇒
     Cenv_bs rd menv s env rmenv renv (rsz+1) bs'``,
   rw[Cenv_bs_def,s_refs_def,good_rd_def,env_renv_def,fmap_rel_def] >> rw[] >> fs[] >>
-  res_tac >>
-  match_mp_tac(GEN_ALL(MP_CANON EVERY2_mono)) >>
-  HINT_EXISTS_TAC >> simp[] >>
-  rpt gen_tac >>
+  TRY (
+    match_mp_tac(GEN_ALL(MP_CANON EVERY2_mono)) >>
+    HINT_EXISTS_TAC >> simp[] >>
+    rpt gen_tac >>
+    BasicProvers.CASE_TAC >>
+    imp_res_tac lookup_ct_imp_incsz >>
+    simp[]) >>
+  first_x_assum(qspec_then`x`mp_tac) >>
+  simp[EVERY2_EVERY,EVERY_MEM,FORALL_PROD,GSYM AND_IMP_INTRO,MEM_ZIP] >>
+  simp_tac(srw_ss()++DNF_ss)[] >>
+  simp[EL_MAP,el_check_def] >>
+  gen_tac >> strip_tac >>
+  disch_then(qspec_then`n`mp_tac) >>
+  simp[AND_IMP_INTRO,CONJ_SYM] >>
+  simp[GSYM AND_IMP_INTRO] >>
   BasicProvers.CASE_TAC >>
-  imp_res_tac lookup_ct_imp_incsz >>
-  simp[])
+  simp[ADD1,EL_APPEND1])
 
 val env_renv_imp_decsz = store_thm("env_renv_imp_decsz",
   ``∀rd rsz bs env renv bs'.
@@ -1503,14 +1513,32 @@ val env_renv_imp_decsz = store_thm("env_renv_imp_decsz",
 val Cenv_bs_imp_decsz = store_thm("Cenv_bs_imp_decsz",
   ``∀rd menv s env rmenv renv rsz bs bs'.
     Cenv_bs rd menv s env rmenv renv (rsz+1) bs ∧
-      (CTLet (rsz+1) ∉ set renv ∪ BIGUNION (IMAGE set (FRANGE rmenv))) ∧
-      (CTDec (LENGTH bs'.stack) ∉ set renv ∪ BIGUNION (IMAGE set (FRANGE rmenv))) ∧
+      (CTLet (rsz+1) ∉ set renv) ∧
+      (CTDec (LENGTH bs'.stack) ∉ set renv) ∧
+      (LENGTH bs'.stack ∉ BIGUNION (IMAGE set (FRANGE rmenv))) ∧
       (∃v p e. bs = bs' with <| stack := v::bs'.stack; pc := p; handler := e |>) ⇒
     Cenv_bs rd menv s env rmenv renv rsz bs'``,
   rw[Cenv_bs_def,fmap_rel_def,s_refs_def,FDOM_DRESTRICT,good_rd_def] >> fs[] >>
-  match_mp_tac env_renv_imp_decsz >>
-  res_tac >> HINT_EXISTS_TAC >>
-  simp[bc_state_component_equality] >>
+  TRY (
+    match_mp_tac env_renv_imp_decsz >>
+    res_tac >> HINT_EXISTS_TAC >>
+    simp[bc_state_component_equality] >>
+    fs[IN_FRANGE] >> metis_tac[]) >>
+  first_x_assum(qspec_then`x`mp_tac)>>
+  simp[env_renv_def,EVERY2_MAP,el_check_def] >>
+  strip_tac >>
+  match_mp_tac(GEN_ALL(MP_CANON EVERY2_MEM_MONO)) >>
+  HINT_EXISTS_TAC >> simp[ADD1,FORALL_PROD] >>
+  fs[EVERY2_EVERY,MEM_ZIP,GSYM LEFT_FORALL_IMP_THM,GSYM AND_IMP_INTRO] >>
+  gen_tac >> strip_tac >> strip_tac >>
+  BasicProvers.CASE_TAC >>
+  ntac 2 (pop_assum mp_tac) >>
+  BasicProvers.CASE_TAC >>
+  simp[AND_IMP_INTRO,CONJ_SYM] >>
+  simp[GSYM AND_IMP_INTRO,EL_APPEND1] >>
+  strip_tac >> spose_not_then strip_assume_tac >>
+  `EL n (rmenv ' x) = LENGTH bs'.stack` by DECIDE_TAC >>
+  `MEM (LENGTH bs'.stack) (rmenv ' x)` by metis_tac[MEM_EL] >>
   fs[IN_FRANGE] >> metis_tac[])
 
 val env_renv_CTLet_bound = store_thm("env_renv_CTLet_bound",
@@ -1534,22 +1562,26 @@ val env_renv_CTDec_bound = store_thm("env_renv_CTDec_bound",
   srw_tac[ARITH_ss][])
 
 val Cenv_bs_CTLet_bound = store_thm("Cenv_bs_CTLet_bound",
-  ``Cenv_bs rd menv s env rmenv renv rsz bs ∧ (CTLet n) ∈ set renv ∪ BIGUNION (IMAGE set (FRANGE rmenv)) ⇒ n ≤ rsz``,
+  ``Cenv_bs rd menv s env rmenv renv rsz bs ∧ (CTLet n) ∈ set renv ⇒ n ≤ rsz``,
   rw[Cenv_bs_def,fmap_rel_def,IN_FRANGE] >>
   match_mp_tac (GEN_ALL env_renv_CTLet_bound) >>
   metis_tac[])
 
 val Cenv_bs_CTDec_bound = store_thm("Cenv_bs_CTDec_bound",
-  ``Cenv_bs rd menv s env rmenv renv rsz bs ∧ (CTDec n) ∈ set renv ∪ BIGUNION (IMAGE set (FRANGE rmenv)) ⇒ n < LENGTH bs.stack``,
+  ``Cenv_bs rd menv s env rmenv renv rsz bs ∧ ((CTDec n) ∈ set renv ∨ n ∈ BIGUNION (IMAGE set (FRANGE rmenv))) ⇒ n < LENGTH bs.stack``,
   rw[Cenv_bs_def,fmap_rel_def,IN_FRANGE] >>
-  match_mp_tac (GEN_ALL env_renv_CTDec_bound) >>
-  metis_tac[])
+  match_mp_tac (GEN_ALL env_renv_CTDec_bound) >-
+    metis_tac[] >>
+  first_x_assum(qspec_then`k`mp_tac) >>
+  simp[o_f_FAPPLY] >> rw[] >>
+  metis_tac[MEM_MAP])
 
 val Cenv_bs_pops = store_thm("Cenv_bs_pops",
   ``∀vs rd menv s env rmenv renv rsz bs bs'.
     Cenv_bs rd menv s env rmenv renv (rsz + LENGTH vs) bs ∧
-    (∀n. (CTLet n) ∈ set renv ∪ BIGUNION (IMAGE set (FRANGE rmenv)) ⇒ n ≤ rsz) ∧
-    (∀n. (CTDec n) ∈ set renv ∪ BIGUNION (IMAGE set (FRANGE rmenv)) ⇒ n < LENGTH bs'.stack) ∧
+    (∀n. (CTLet n) ∈ set renv ⇒ n ≤ rsz) ∧
+    (∀n. (CTDec n) ∈ set renv ⇒ n < LENGTH bs'.stack) ∧
+    (∀n. n ∈ BIGUNION (IMAGE set (FRANGE rmenv)) ⇒ n < LENGTH bs'.stack) ∧
     (∃p e. bs = bs' with <| stack := vs ++ bs'.stack; pc := p; handler := e|>)
     ⇒ Cenv_bs rd menv s env rmenv renv rsz bs'``,
   Induct >> rw[] >- ( fs[Cenv_bs_def,s_refs_def,good_rd_def,fmap_rel_def,env_renv_def] >> fs[]) >>
@@ -1562,7 +1594,7 @@ val Cenv_bs_pops = store_thm("Cenv_bs_pops",
   qexists_tac`y` >>
   unabbrev_all_tac >>
   fsrw_tac[ARITH_ss][ADD1,bc_state_component_equality] >>
-  conj_tac >> conj_tac >>
+  conj_tac >> TRY conj_tac >>
   spose_not_then strip_assume_tac >>
   TRY(BasicProvers.VAR_EQ_TAC) >>
   res_tac >> fsrw_tac[ARITH_ss][] )
@@ -1624,6 +1656,10 @@ val Cenv_bs_append_code = store_thm("Cenv_bs_append_code",
   fs[Cenv_bs_def,EVERY2_EVERY,EVERY_MEM,FORALL_PROD,s_refs_def,env_renv_def,fmap_rel_def] >> rw[] >>
   res_tac >>
   BasicProvers.CASE_TAC >> fs[] >>
+  TRY (
+    qmatch_assum_rename_tac`MEM (a,b) X`["X"]>>
+    first_x_assum(qspecl_then[`b`,`a`]mp_tac) >>
+    simp[] >> strip_tac) >>
   match_mp_tac Cv_bv_l2a_mono_mp >>
   qexists_tac `mk_pp rd bs` >>
   rw[] >> metis_tac[bc_find_loc_aux_append_code])
@@ -1635,12 +1671,25 @@ val Cenv_bs_FUPDATE = store_thm("Cenv_bs_FUPDATE",
     (bs' = bs with stack := bv::bs.stack)
     ⇒
     Cenv_bs rd menv s (v::env) rmenv ((CTLet (sz0 + 1))::env0) (sz0 + 1) bs'``,
-  reverse(rw[Cenv_bs_def,s_refs_def]) >> fs[el_check_def] >- fs[good_rd_def] >> (
-  fs[EVERY2_EVERY,EVERY_MEM,FORALL_PROD,env_renv_def,fmap_rel_def,el_check_def] >>
-  rpt strip_tac >> res_tac >>
-  pop_assum mp_tac >> BasicProvers.CASE_TAC >>
-  imp_res_tac lookup_ct_imp_incsz >>
-  simp[] ))
+  reverse(reverse(rw[Cenv_bs_def,s_refs_def]) >> fs[el_check_def] >- fs[good_rd_def]) >- (
+    fs[EVERY2_EVERY,EVERY_MEM,FORALL_PROD,env_renv_def,fmap_rel_def,el_check_def] >>
+    rpt strip_tac >> res_tac >>
+    pop_assum mp_tac >> BasicProvers.CASE_TAC >>
+    imp_res_tac lookup_ct_imp_incsz >>
+    simp[] ) >>
+  fsrw_tac[DNF_ss][fmap_rel_def] >> rw[] >>
+  first_x_assum(qspec_then`x`mp_tac) >>
+  simp[] >>
+  simp[env_renv_def] >> strip_tac >>
+  match_mp_tac(GEN_ALL(MP_CANON EVERY2_MEM_MONO)) >>
+  HINT_EXISTS_TAC >> simp[ADD1,FORALL_PROD] >>
+  fs[EVERY2_EVERY,MEM_ZIP,GSYM LEFT_FORALL_IMP_THM,GSYM AND_IMP_INTRO,EL_MAP,el_check_def,ADD1] >>
+  gen_tac >> strip_tac >> strip_tac >>
+  BasicProvers.CASE_TAC >>
+  ntac 2 (pop_assum mp_tac) >>
+  BasicProvers.CASE_TAC >>
+  simp[AND_IMP_INTRO,CONJ_SYM] >>
+  simp[GSYM AND_IMP_INTRO,EL_APPEND1])
 
 val Cenv_bs_FUPDATE_LIST = store_thm("Cenv_bs_FUPDATE_LIST",
   ``∀vs rd menv s env rmenv cenv sz bs bs bvs bs' env' cenv' sz'.
@@ -1716,7 +1765,7 @@ val Cenv_bs_change_store = store_thm("Cenv_bs_change_store",
     Cenv_bs rd' menv s' env rmenv renv rsz bs'``,
   rw[Cenv_bs_def,EVERY2_EVERY,EVERY_MEM,FORALL_PROD,fmap_rel_def] >>
   match_mp_tac (GEN_ALL env_renv_change_store) >>
-  metis_tac[])
+  metis_tac[o_f_FAPPLY])
 
 val retbc_thm = store_thm("retbc_thm",
   ``∀bs bc0 bc1 bv vs benv ret args x st bs'.
@@ -1957,7 +2006,7 @@ val compile_bindings_thm = store_thm("compile_bindings_thm",
 
 val Cenv_bs_bind_fv = store_thm("Cenv_bs_bind_fv",
   ``∀menv rmenv cenv ccenv benv bve ret bvs a st fenv defs ix recs envs env pp rd bs s vs az e l e'.
-    fmap_rel (env_renv rd 0 bs) menv rmenv ∧
+    fmap_rel (env_renv rd 0 bs) menv (MAP CTDec o_f rmenv) ∧
     (cenv = MAP CTEnv ccenv) ∧
     (benv = Block 0 bve) ∧
     (bs.stack = benv::CodePtr ret::(REVERSE bvs)++(Block closure_tag [CodePtr a;benv])::st) ∧
@@ -2053,13 +2102,14 @@ val code_env_cd_def = Define`
       (code = bc0 ++ Label l :: (REVERSE cc) ++ bc1)`
 
 val Cenv_bs_with_irr = store_thm("Cenv_bs_with_irr",
-  ``∀rd s env cenv sz bs bs'.
-    Cenv_bs rd s env cenv sz bs ∧
+  ``∀rd menv s env rmenv cenv sz bs bs'.
+    Cenv_bs rd menv s env rmenv cenv sz bs ∧
     (bs'.stack = bs.stack) ∧ (bs'.refs = bs.refs) ∧
     (bs'.code = bs.code) ∧ (bs'.inst_length = bs.inst_length)
     ⇒
-    Cenv_bs rd s env cenv sz bs'``,
-  rw[Cenv_bs_def,s_refs_def,good_rd_def])
+    Cenv_bs rd menv s env rmenv cenv sz bs'``,
+  rw[Cenv_bs_def,s_refs_def,good_rd_def,env_renv_def,fmap_rel_def] >>
+  rfs[o_f_FAPPLY])
 
 val s_refs_with_irr = store_thm("s_refs_with_irr",
   ``∀rd s bs bs'.
